theories/Erase/Comp.v
@@ -1,0 +1,460 @@
+From Coq Require Import ZArith.ZArith Sets.Ensembles Lists.List.
+From compcert.lib Require Export Maps.
+From CertiCoq.LambdaANF Require Import Ensembles_util map_util set_util List_util tactics.
+From CertiCoq.Libraries Require Import maps_util.
+Import ListNotations.
+Require Import Lia.
+From Hammer Require Import Hammer Tactics Reflect.
+
+From Common Require Import Util.
+From LambdaANF Require Import ANF.
+From LambdaWeb Require Import ANF.
+From Erase Require Import Erase.
+
+Module A0 := LambdaANF.ANF.
+Module A1 := LambdaWeb.ANF.
+
+(* Cross-language Compositionality *)
+
+(* Adequacy *)
+Theorem adequacy e1 e2:
+  trans_correct_top e1 e2 ->
+  forall ρ1 ρ2,
+    wf_env ρ1 ->
+    (forall k, G_top k (A1.occurs_free e1) ρ1 (A0.occurs_free e2) ρ2) ->
+    forall j1 r1,
+      A1.bstep_fuel true ρ1 e1 j1 r1 ->
+      exists j2 r2,
+        A0.bstep_fuel ρ2 e2 j2 r2 /\
+        (forall k, R k r1 r2).
+Proof.
+  intros.
+  unfold trans_correct_top in H.
+  destruct H as [HS HT].
+
+  assert (HE : E true j1 ρ1 e1 ρ2 e2) by (eapply (HT j1); eauto).
+  edestruct (HE j1) as [j2 [r2 [Hstep2 HR]]]; eauto.
+  eexists; eexists; split; eauto.
+
+  intros.
+  assert (HE' : E true (j1 + k) ρ1 e1 ρ2 e2) by (eapply HT; eauto).
+  edestruct (HE' j1) as [j2' [r2' [Hstep2' HR']]]; eauto; try lia.
+
+  rewrite_math (j1 + k - j1 = k).
+  rewrite_math (j1 - j1 = 0).
+
+  destruct r2; destruct r2'; destruct r1;
+    simpl in *; auto; try contradiction.
+
+  edestruct (A0.bstep_fuel_deterministic v v0 Hstep2 Hstep2'); subst; eauto.
+Qed.
+
+(* Behavioral Refinement *)
+Inductive val_ref : A1.wval -> A0.val -> Prop :=
+| Ref_Tag :
+  forall w v1 v2,
+    (w \in Exposed) ->
+    val_ref' v1 v2 ->
+    val_ref (Tag w v1) v2
+
+with val_ref' : A1.val -> A0.val -> Prop :=
+| Ref_Vfun :
+  forall f1 ρ1 xs1 e1 f2 ρ2 xs2 e2,
+    val_ref' (A1.Vfun f1 ρ1 xs1 e1) (A0.Vfun f2 ρ2 xs2 e2)
+
+| Ref_Vconstr_nil :
+  forall c,
+    val_ref' (A1.Vconstr c []) (A0.Vconstr c [])
+
+| Ref_Vconstr_cons :
+  forall c v1 v2 vs1 vs2,
+    val_ref v1 v2 ->
+    val_ref' (A1.Vconstr c vs1) (A0.Vconstr c vs2) ->
+    val_ref' (A1.Vconstr c (v1 :: vs1)) (A0.Vconstr c (v2 :: vs2)).
+
+Hint Constructors val_ref : core.
+Hint Constructors val_ref' : core.
+
+Scheme val_ref_mut := Induction for val_ref Sort Prop
+with val_ref'_mut := Induction for val_ref' Sort Prop.
+
+Lemma val_ref_Vconstr c w vs1 vs2 :
+  (w \in Exposed) ->
+  Forall2 val_ref vs1 vs2 ->
+  val_ref (Tag w (A1.Vconstr c vs1)) (A0.Vconstr c vs2).
+Proof.
+  intros.
+  induction H0; simpl; auto.
+  fcrush.
+Qed.
+
+Lemma V_val_ref {v1 v2} :
+  wf_val v1 ->
+  exposed v1 ->
+  (forall i, V i v1 v2) ->
+  val_ref v1 v2.
+Proof.
+  intros H.
+  revert v2.
+  induction H using wf_val_mut with (P0 := fun v1 wf =>
+                                             forall (v2 : A0.val) w,
+                                               (w \in Exposed) ->
+                                               (match v1 with
+                                                | Vfun _ _ _ _ => True
+                                                | Vconstr c vs1 => Forall exposed vs1
+                                                end) ->
+                                               (forall i, (V i (Tag w v1) v2)) ->
+                                               match v1, v2 with
+                                               | A1.Vfun _ _ _ _, A0.Vfun _ _ _ _ => True
+                                               | A1.Vconstr c1 vs1, A0.Vconstr c2 vs2  =>
+                                                   c1 = c2 /\ Forall2 val_ref vs1 vs2
+                                               | _ , _ => False
+                                               end)
+                                    (P1 := fun ρ wf => True);
+    intros; simpl in *; eauto.
+  - inv H.
+    + specialize (IHwf_val v2 _ H2).
+      destruct v2.
+      destruct v; try contradiction; subst; auto.
+      fcrush.
+    + specialize (IHwf_val v2 _ H3 H4).
+      destruct v2.
+      destruct v; try contradiction; subst; auto.
+      * edestruct IHwf_val as [Heqc Hval]; eauto; subst.
+        eapply val_ref_Vconstr; eauto.
+  - destruct v2.
+    destruct v; auto;
+      destruct (H1 0) as [_ [_ [Hw H']]]; subst; auto; contradiction.
+    specialize (H1 0).
+    sfirstorder.
+  - destruct v2.
+    + specialize (H1 0); sfirstorder.
+    + specialize (H1 0); simpl in *;
+        destruct H1 as [Hc Hlen].
+      sauto.
+  - destruct v2.
+    + specialize (H2 0); sfirstorder.
+    + pose proof H2 as HV.
+      specialize (H2 1); simpl in *;
+        destruct H2 as [Hv1 [Hc HV']]; subst;
+          split; auto.
+      inv HV'.
+      clear H4 H6.
+      assert (HV' : forall i, V i v y /\ V i (A1.Tag w0 (A1.Vconstr c0 vs)) (A0.Vconstr c0 l')).
+      {
+        intros.
+        specialize (HV (S i)).
+        destruct i; simpl in *;
+          destruct HV as [_ [_ HFV]];
+          inv HFV.
+          - inv Hv1.
+            inv H1.
+            inv H6.
+            repeat (split; auto).
+            + eapply Forall2_length; eauto.
+          - inv Hv1.
+            inv H1.
+            inv H6.
+            repeat (split; auto).
+            eapply V_mono_Forall with (S i); eauto.
+      }
+
+      assert (HV0 : forall i, V i v y) by (intros; destruct (HV' i); auto).
+      assert (HV1 : forall i, V i (A1.Tag w0 (A1.Vconstr c0 vs)) (A0.Vconstr c0 l')) by (intros; destruct (HV' i); auto).
+
+      inv H1.
+      constructor; auto.
+      fcrush.
+Qed.
+
+Lemma R_res_val_ref {v1 v2} :
+  wf_val v1 ->
+  exposed v1 ->
+  (forall i, R i (A1.Res v1) (A0.Res v2)) ->
+  val_ref v1 v2.
+Proof. intros; eapply V_val_ref; eauto. Qed.
+
+(* Linking Compat Lemmas *)
+
+(* [trans_correct] is stronger than [trans_correct_top] due to [G_top] *)
+Lemma trans_correct_trans_correct_top e1 e2 :
+  A0.occurs_free e2 \subset A1.occurs_free e1 ->
+  trans_correct (A1.occurs_free e1) e1 e2 ->
+  trans_correct_top e1 e2.
+Proof.
+  unfold trans_correct_top, trans_correct.
+  intros.
+  split; auto; intros.
+  eapply H0; eauto.
+  eapply G_top_G; eauto.
+Qed.
+
+(* Top-level Environment Lemmas *)
+Lemma G_top_get_list {i Γ1 ρ1 Γ2 ρ2} :
+  G_top i Γ1 ρ1 Γ2 ρ2 ->
+  forall xs,
+    (FromList xs) \subset Γ1 ->
+    exists vs1 vs2,
+      get_list xs ρ1 = Some vs1 /\
+      get_list xs ρ2 = Some vs2 /\
+      Forall2 (V i) vs1 vs2.
+Proof.
+  unfold G_top.
+  intros HG xs.
+  destruct HG as [Hr2 [HS HG]].
+  induction xs; simpl; intros.
+  - eexists; eexists; repeat split; eauto.
+  - rewrite FromList_cons in H.
+    edestruct IHxs as [vs1 [vs2 [Heqvs1 [Heqvs2 HVs]]]].
+    eapply Included_trans; eauto.
+    apply Included_Union_r.
+
+    destruct (HG a) as [v1 [v2 [Heqv1 [Heqv2 [Hex HV]]]]].
+    unfold Ensembles.Included, Ensembles.In, FromList in *.
+    eapply H; eauto.
+    apply Union_introl; auto.
+
+    rewrite Heqv1.
+    rewrite Heqvs1.
+    rewrite Heqv2.
+    rewrite Heqvs2.
+    exists (v1 :: vs1), (v2 :: vs2); split; auto.
+Qed.
+
+Lemma G_top_set {i Γ1 ρ1 Γ2 ρ2}:
+  G_top i Γ1 ρ1 Γ2 ρ2 ->
+  forall {x v1 v2},
+    exposed v1 ->
+    V i v1 v2 ->
+    G_top i (x |: Γ1) (M.set x v1 ρ1) (x |: Γ2) (M.set x v2 ρ2).
+Proof.
+  unfold G_top.
+  intros.
+  destruct H as [Hr2 [HS HG]].
+  split.
+  eapply wf_env_set; eauto.
+  eapply V_wf_val_l; eauto.
+
+  split.
+  apply Included_Union_compat; auto.
+  apply Included_refl.
+
+  intros.
+  destruct (M.elt_eq x0 x); subst.
+  - repeat rewrite M.gss.
+    eexists; eexists; repeat split; eauto.
+  - repeat (rewrite M.gso; auto).
+    inv H.
+    inv H2; contradiction.
+    eapply HG; eauto.
+Qed.
+
+Lemma G_top_set_lists {i Γ1 ρ1 Γ2 ρ2}:
+  G_top i Γ1 ρ1 Γ2 ρ2 ->
+  forall {xs vs1 vs2 ρ3 ρ4},
+    Forall2 (V i) vs1 vs2 ->
+    Forall exposed vs1 ->
+    set_lists xs vs1 ρ1 = Some ρ3 ->
+    set_lists xs vs2 ρ2 = Some ρ4 ->
+    G_top i (FromList xs :|: Γ1) ρ3 (FromList xs :|: Γ2) ρ4.
+Proof.
+  unfold G_top.
+  intros HG xs.
+  induction xs; simpl; intros.
+  - destruct vs1; try discriminate.
+    destruct vs2; try discriminate.
+    inv H1; inv H2.
+    destruct HG as [Hr2 [HS HG]].
+    repeat (split; auto); intros.
+    apply Included_Union_compat; auto.
+    apply Included_refl.
+    inv H1.
+    inv H2.
+    eapply HG; eauto.
+  - destruct vs1; try discriminate.
+    destruct vs2; try discriminate.
+    destruct (set_lists xs vs1 ρ1) eqn:Heq1; try discriminate.
+    destruct (set_lists xs vs2 ρ2) eqn:Heq2; try discriminate.
+    inv H; inv H0; inv H1; inv H2.
+    destruct HG as [Hr1 [HS HG]].
+
+    split.
+    eapply wf_env_set; eauto.
+    eapply (wf_env_set_lists _ Hr1 vs1 xs); eauto.
+    eapply V_wf_val_Forall_l; eauto.
+    eapply V_wf_val_l; eauto.
+
+    split.
+    apply Included_Union_compat; auto.
+    apply Included_refl.
+
+    intros.
+    destruct (M.elt_eq x a); subst.
+    + repeat rewrite M.gss in *; eauto.
+      eexists; eexists; split; eauto.
+    + repeat (rewrite M.gso in *; auto).
+      edestruct IHxs as [v1' [v2' [Heqv1' [Heqv2' [Hex HV']]]]]; eauto.
+      eapply not_In_cons_Union; eauto.
+Qed.
+
+(* Monotonicity Lemma *)
+Lemma G_top_mono {Γ1 Γ2 ρ1 ρ2} i j:
+  G_top i Γ1 ρ1 Γ2 ρ2 ->
+  j <= i ->
+  G_top j Γ1 ρ1 Γ2 ρ2.
+Proof.
+  unfold G_top.
+  intros.
+  destruct H as [Hr2 [HS HG]].
+  repeat (split; auto); intros.
+  edestruct HG as [v1 [v2 [Heqv1 [Heqv2 [Hex HV]]]]]; eauto.
+  eexists; eexists; repeat split; eauto.
+  apply V_mono with i; eauto.
+Qed.
+
+(* Compatibility Lemmas *)
+Lemma Vfun_V_top e e' :
+  trans_correct_top e e' ->
+  forall i f w xs Γ1 Γ2 ρ1 ρ2,
+    wf_env ρ1 ->
+    G_top i Γ1 ρ1 Γ2 ρ2 ->
+    (w \in Exposed) ->
+    A1.occurs_free e \subset (FromList xs :|: (f |: Γ1)) ->
+    A0.occurs_free e' \subset (FromList xs :|: (f |: Γ2)) ->
+    V i (Tag w (A1.Vfun f ρ1 xs e)) (A0.Vfun f ρ2 xs e').
+Proof.
+  unfold trans_correct_top.
+  intros [HS He] i.
+  induction i; simpl; intros; auto.
+  repeat (split; auto); intros.
+  destruct (exposed_reflect w); try contradiction.
+
+  apply (He (i - (i - j)) ρ3 ρ4); auto.
+  eapply G_top_subset with (Γ1 := FromList xs :|: (f |: Γ1)) (Γ2 := FromList xs :|: (f |: Γ2)); eauto.
+  eapply G_top_set_lists; eauto.
+  eapply G_top_set; eauto.
+  eapply G_top_mono; eauto; try lia.
+  apply V_mono with i; try lia.
+  eapply IHi with (Γ2 := Γ2); eauto.
+  apply G_top_mono with (S i); eauto; lia.
+Qed.
+
+Lemma free_fun_compat e e' f w k k' xs :
+  A0.occurs_free e' \subset A1.occurs_free e ->
+  A0.occurs_free k' \subset A1.occurs_free k ->
+  A0.occurs_free (A0.Efun f xs e' k') \subset A1.occurs_free (A1.Efun f w xs e k).
+Proof.
+  unfold Ensembles.Included, Ensembles.In.
+  intros.
+  inv H1; auto.
+Qed.
+
+Lemma fun_compat_top e e' k k' f w xs :
+  (w \in Exposed) ->
+  trans_correct_top e e' ->
+  trans_correct_top k k' ->
+  trans_correct_top (A1.Efun f w xs e k) (A0.Efun f xs e' k').
+Proof.
+  unfold trans_correct_top, E, E'.
+  intro Hex.
+  intros.
+  destruct H.
+  destruct H0.
+  split; intros.
+  eapply free_fun_compat; eauto.
+
+  pose proof H3 as HG.
+  destruct H3 as [Hr2 [HS HG']].
+  inv H5.
+  - exists 0, A0.OOT; split; simpl; eauto.
+  - inv H3.
+    edestruct (H2 (i - 1) (M.set f (Tag w (A1.Vfun f ρ1 xs e)) ρ1) (M.set f (A0.Vfun f ρ2 xs e') ρ2)) with (j1 := c) (r1 := r1) as [j2 [r2 [Hk2 Rr]]]; eauto; try lia.
+    + eapply G_top_subset with (Γ1 := (f |: (A1.occurs_free (A1.Efun f w xs e k)))) (Γ2 := (f |: (A0.occurs_free (A0.Efun f xs e' k')))); eauto.
+      * eapply G_top_set; eauto.
+        eapply G_top_mono; eauto; try lia.
+        eapply Vfun_V_top with (Γ1 := (A1.occurs_free (A1.Efun f w xs e k))) (Γ2 := (A0.occurs_free (A0.Efun f xs e' k'))); eauto.
+        -- unfold trans_correct_top.
+           split; auto.
+        -- eapply G_top_mono; eauto; try lia.
+        -- eapply A1.free_fun_e_subset; eauto.
+        -- eapply A0.free_fun_e_subset; eauto.
+      * eapply A1.free_fun_k_subset; eauto.
+    + exists (S j2), r2; split; auto.
+      apply R_mono with ((i - 1) - c); try lia; auto.
+Qed.
+
+Lemma free_letapp_compat k k' f w x xs :
+  A0.occurs_free k' \subset A1.occurs_free k ->
+  A0.occurs_free (A0.Eletapp x f xs k') \subset A1.occurs_free (A1.Eletapp x f w xs k).
+Proof.
+  unfold Ensembles.Included, Ensembles.In.
+  intros.
+  inv H0; auto.
+Qed.
+
+Lemma letapp_compat_top k k' xs x f w :
+  (w \in Exposed) ->
+  trans_correct_top k k' ->
+  trans_correct_top (A1.Eletapp x f w xs k) (A0.Eletapp x f xs k').
+Proof.
+  unfold trans_correct_top, E, E'.
+  intro Hex.
+  intros.
+  destruct H.
+  split; intros.
+  eapply free_letapp_compat; eauto.
+
+  pose proof H1 as HG.
+  destruct H1 as [Hr2 [HS HG']].
+  inv H3.
+  - exists 0, A0.OOT; split; simpl; auto.
+  - inv H1.
+    + edestruct (HG' f) as [fv1 [fv2 [Heqfv1 [Heqfv2 [Hexfv HVf]]]]]; eauto.
+      rewrite Heqfv1 in H9; inv H9.
+      destruct i.
+      inv H2.
+      destruct fv2; simpl in HVf.
+      2 : { inv HVf; contradiction. }
+
+      destruct HVf as [Hfv2 [Hlen HV]]; subst.
+
+      edestruct (G_top_get_list HG xs) as [vs1 [vs2 [Heqvs1 [Heqvs2 HVvs]]]].
+      eapply A1.free_letapp_xs_subset; eauto.
+
+      rewrite Heqvs1 in H10; inv H10.
+
+      destruct (set_lists_length3 (M.set v0 (A0.Vfun v0 t l e0) t) l vs2) as [ρ4 Heqρ4].
+      unfold wval in *.
+      rewrite <- (Forall2_length _ _ _ HVvs).
+      rewrite <- (set_lists_length_eq _ _ _ _ H13); auto.
+
+      unfold E' in HV.
+      edestruct (HV i vs vs2 ρ'' ρ4) with (j1 := c0) as [j2 [r2 [He0 HR]]]; eauto; try lia.
+      * intros.
+        destruct H15; auto.
+      * eapply V_mono_Forall; eauto; lia.
+      * destruct r2; simpl in HR; try contradiction.
+        edestruct (H0 (i - c0) (M.set x v ρ1) (M.set x v1 ρ2)) with (j1 := c') as [j3 [r3 [He1 HR']]]; eauto; try lia.
+        eapply G_top_subset with (Γ1 := x |: (A1.occurs_free (A1.Eletapp x f w xs k))) (Γ2 := x |: (A0.occurs_free (A0.Eletapp x f xs k'))); eauto.
+        eapply G_top_set; eauto.
+        eapply G_top_mono; eauto; lia.
+        -- destruct H15; auto.
+        -- eapply V_mono; eauto; try lia.
+        -- eapply A1.free_letapp_k_subset; eauto.
+        -- exists (S (j2 + j3)), r3; split; eauto.
+           eapply R_mono; eauto; lia.
+    + eexists; exists A0.OOT; split; simpl; eauto.
+Qed.
+
+(* Linking Preservation *)
+Lemma preserves_linking f w x e1 e2 e1' e2' :
+  (w \in Exposed) ->
+  trans_correct_top e1 e2 ->
+  trans_correct_top e1' e2' ->
+  trans_correct_top (A1.link f w x e1 e1') (A0.link f x e2 e2').
+Proof.
+  unfold A0.link, A1.link.
+  intros.
+  eapply fun_compat_top; eauto.
+  eapply letapp_compat_top; eauto.
+Qed.
